examples/low-level/FStar.Buffer.fst
@@ -275,7 +275,9 @@ val upd: #a:Type -> b:buffer a -> n:u32 -> z:a -> STL unit
     /\ modifies_1 b h0 h1
     (* /\ modifies_one (frameOf b) h0 h1 *)
     (* /\ modifies_buf (frameOf b) (only b) h0 h1 *)
-    /\ sel h1 b = Seq.upd (sel h0 b) (idx b + v n) z))
+    /\ sel h1 b = Seq.upd (sel h0 b) (idx b + v n) z
+    /\ get h1 b (v n) = z
+    /\ (forall (i:nat). {:pattern (get h1 b (v n))} (i < length b /\ i <> v n) ==> get h1 b i = get h0 b i) ))
 let upd #a b n z =
   let s = !b.content in
   let s = Seq.upd s (v b.idx + v n) z in
